Consolidate term functions.

cryptis/core/term/base.v
@@ -5,6 +5,8 @@ From Stdlib Require Import ZArith.ZArith Lia.
 From stdpp Require Import sorting gmap.
 From cryptis.lib Require Import list_sort mathcomp_compat.
 From iris.heap_lang Require locations.
+From iris.heap_lang Require Import notation.
+From iris.heap_lang Require Import primitive_laws.
 From cryptis.core Require Export pre_term.
 
 (* [PreTerm.wf_term] is the [wf] boolean fixpoint; keep [simpl] from unfolding it
@@ -222,6 +224,7 @@ Lemma unfold_term_inj : injective unfold_term.
 Proof. exact: can_inj unfold_termK. Qed.
 
 Global Instance unfold_term_inj_inst : Inj (=) (=) unfold_term := unfold_term_inj.
+
 
 Implicit Types (t k : term) (ts : list term).
 
@@ -619,7 +622,7 @@ Lemma unfold_merge_sort s :
   unfold_term <$> merge_sort term_order s = merge_sort pt_order (unfold_term <$> s).
 Proof. apply: merge_sort_fmap => x y; rewrite /term_order; reflexivity. Qed.
 
-Lemma exps_TExpN t ts :
+Lemma exps_TExpN_sort t ts :
   Forall (fun t => negb (is_mul t)) ts ->
   exps (TExpN t ts) = merge_sort term_order (cancel_invs (exps t ++ ts)).
 Proof.
@@ -664,7 +667,7 @@ Qed.
 Lemma is_exp_unfold t : is_exp t = PreTerm.is_exp (unfold_term t).
 Proof. by case: t. Qed.
 
-Lemma is_exp_base t : negb (is_exp (base t)).
+Lemma is_exp_base_bool t : negb (is_exp (base t)).
 Proof.
 rewrite is_exp_unfold unfold_base.
 exact: (PreTerm.base_Nexp _ (wf_unfold_term t)).
@@ -690,13 +693,13 @@ move=> eb ee; rewrite -(base_expsK t1) -(base_expsK t2) eb.
 exact: TExpN_perm.
 Qed.
 
-Lemma base_expN t : negb (is_exp t) -> base t = t.
+Lemma base_expN_bool t : negb (is_exp t) -> base t = t.
 Proof.
 rewrite is_exp_unfold=> tNX; apply: unfold_term_inj.
 by rewrite unfold_base (PreTerm.base_expN _ tNX).
 Qed.
 
-Lemma exps_expN t : negb (is_exp t) -> exps t = [].
+Lemma exps_expN_bool t : negb (is_exp t) -> exps t = [].
 Proof.
 rewrite is_exp_unfold=> tNX; apply: (inj (fmap unfold_term)).
 by rewrite unfold_exps (PreTerm.exps_expN _ tNX).
@@ -790,7 +793,7 @@ move=> /negb_True Nm E; apply: Nm; rewrite E is_mul_unfold unfold_TMulN.
 by [].
 Qed.
 
-Lemma invs_canceled1 t : invs_canceled [t] <-> t ≠ TMulN [].
+Lemma invs_canceled1_iff t : invs_canceled [t] <-> t ≠ TMulN [].
 Proof.
 rewrite invs_canceledE Forall_singleton not_elem_of_cons; split.
 - by move=> [H _] E; apply: H; rewrite E TInv_fixed.
@@ -799,7 +802,7 @@ rewrite invs_canceledE Forall_singleton not_elem_of_cons; split.
 Qed.
 
 Lemma invs_canceled_Nmul1 {t} : negb (is_mul t) -> invs_canceled [t].
-Proof. by move=> Nm; apply/invs_canceled1; exact: Nmul_neq_unit. Qed.
+Proof. by move=> Nm; apply/invs_canceled1_iff; exact: Nmul_neq_unit. Qed.
 
 Lemma invs_canceled_cons {t ts} :
   negb (is_mul t) ->
@@ -818,7 +821,7 @@ move=> Nm; rewrite !invs_canceledP; split.
     by rewrite -Heq.
 Qed.
 
-Lemma invs_canceled2 t1 t2 :
+Lemma invs_canceled2_iff t1 t2 :
   invs_canceled [t1 ; t2] <-> (TInv t1 ≠ t2 /\ TMulN [] ∉ [t1; t2]).
 Proof.
 have NE2 : forall (x a b : term), x ∉ [a;b] <-> x ≠ a /\ x ≠ b.
@@ -1066,8 +1069,8 @@ have e1 : tsize t1 = (if bool_decide (exps t1 ≠ []) then 1 else 0)
                      + (if bool_decide (1 < length (exps t1)) then 1 else 0)
                      + tsize (base t1) + sum_list_with tsize (exps t1).
   by rewrite -{1}(base_expsK t1)
-     (tsize_TExpN _ _ (is_exp_base t1) (atom_exps t1) (invs_canceled_exps t1)).
-rewrite TExp_expsE (tsize_TExpN _ _ (is_exp_base t1) atom canc).
+     (tsize_TExpN _ _ (is_exp_base_bool t1) (atom_exps t1) (invs_canceled_exps t1)).
+rewrite TExp_expsE (tsize_TExpN _ _ (is_exp_base_bool t1) atom canc).
 rewrite length_app sum_list_with_app /=.
 have g1 := tsize_gt0 (base t1).
 have g2 := tsize_gt0 t2.
@@ -1101,7 +1104,7 @@ Lemma TExpN_injr t ts1 ts2 :
   cancel_invs ts1 ≡ₚ cancel_invs ts2.
 Proof.
 move => atom1 atom2 /(f_equal exps).
-rewrite (exps_TExpN _ _ atom1) (exps_TExpN _ _ atom2) => Hsort.
+rewrite (exps_TExpN_sort _ _ atom1) (exps_TExpN_sort _ _ atom2) => Hsort.
 have Hperm : cancel_invs (exps t ++ ts1) ≡ₚ cancel_invs (exps t ++ ts2).
   apply: (merge_sort_eq_Permutation term_order); exact: Hsort.
 by apply/(perm_cancel_invs_catl _ _ _ atom1 atom2 (atom_exps t)); exact: Hperm.
@@ -1158,7 +1161,7 @@ case Hm: (is_mul t1).
   have Hic1 := @invs_canceled_count t1 (exps t2) (invs_canceled_exps t2).
   rewrite -/(count_exp_nat t1 t2) -/(count_exp_nat (TInv t1) t2) in Hic1.
   rewrite /count_exp_nat TExp_expsE TExpN_catC.
-  rewrite (exps_TExpN _ _ atom) (exps_expN _ (is_exp_base t2)) app_nil_l count_mem_merge_sort.
+  rewrite (exps_TExpN_sort _ _ atom) (exps_expN_bool _ (is_exp_base_bool t2)) app_nil_l count_mem_merge_sort.
   rewrite (count_cancel _ _ Nmt1 atom) !count_mem_app !single KeyE.
   rewrite -/(count_exp_nat t1 t2) -/(count_exp_nat (TInv t1) t2).
   case: (decide (t1 = TInv t3)) => [e|ne].
@@ -1197,7 +1200,7 @@ Variant count_exp_nat_TExp_spec t1 t2 t3 : nat -> Type :=
 : count_exp_nat_TExp_spec t1 t2 t3 (pred (count_exp_nat t1 t2))
 
 | CountExpTExpDiff
-  of t1 <> t3 & t1 <> TInv t3
+  of t1 ≠ t3 & t1 ≠ TInv t3
 : count_exp_nat_TExp_spec t1 t2 t3 (count_exp_nat t1 t2).
 
 Lemma count_exp_nat_TExpP t1 t2 t3 :
@@ -1261,7 +1264,7 @@ Lemma exps_Nnil t : is_exp t -> exps t ≠ [].
 Proof.
 move => xt E.
 have Hexp : is_exp t = negb (bool_decide (exps t = [])).
-  by rewrite -{1}(base_expsK t) (is_exp_TExpN _ _ (is_exp_base t) (atom_exps t) (invs_canceled_exps t)).
+  by rewrite -{1}(base_expsK t) (is_exp_TExpN _ _ (is_exp_base_bool t) (atom_exps t) (invs_canceled_exps t)).
 move: xt; rewrite Hexp E /=; by move=> [].
 Qed.
 
@@ -1294,9 +1297,9 @@ Proof.
 move => t'_t.
 have en : exps t ≠ [] by move=> e; rewrite e elem_of_nil in t'_t.
 have xt : is_exp t.
-  case E: (is_exp t) => //; move: en; rewrite (exps_expN _ _) //; by rewrite E.
+  case E: (is_exp t) => //; move: en; rewrite (exps_expN_bool _ _) //; by rewrite E.
 rewrite -{1}(base_expsK t)
-  (tsize_TExpN _ _ (is_exp_base t) (atom_exps t) (invs_canceled_exps t)).
+  (tsize_TExpN _ _ (is_exp_base_bool t) (atom_exps t) (invs_canceled_exps t)).
 have Hle := tsize_in_sumn _ _ t'_t.
 have Hb := tsize_gt0 (base t).
 rewrite (bool_decide_eq_true_2 (exps t ≠ []) en) /=; lia.
@@ -1431,7 +1434,7 @@ case: t IH build => [n|t1 t2|a|kt t|k t|t|pt wf nf] IH build.
     rewrite -(base_expsK t).
     apply: H8.
     * apply: IH; exact: tsize_base_lt.
-    * exact: is_exp_base.
+    * exact: is_exp_base_bool.
     * by apply: build => t' t'_t; exact: (tsize_exps_lt _ _ t'_t).
     * exact: atom_exps.
     * exact: exps_Nnil xt.
@@ -1472,3 +1475,1241 @@ Definition func_of_term t :=
   | TKey kt _ => Some (func_of_key_type kt)
   | _ => None
   end.
+
+Set Implicit Arguments.
+Unset Strict Implicit.
+Unset Printing Implicit Defensive.
+
+(*
+Lemma tsize_TExpN_exp t ts t' : t' ∈ ts → tsize t' < tsize (TExpN t ts).
+Proof.
+elim: ts => [|t'' ts IH].
+- by rewrite elem_of_nil.
+- rewrite elem_of_cons; case => [->|/IH t'_ts].
+  + by case: (tsize_TExpN_lt t ts t'').
+  + case: (tsize_TExpN_lt t ts t'') => ??; lia.
+Qed.
+*)
+
+(*
+Lemma tsize_TExp_exp t1 t2 : tsize t2 < tsize (TExp t1 t2).
+Proof. apply: tsize_TExpN_exp. rewrite elem_of_cons. by auto. Qed.
+*)
+
+Canonical termO := leibnizO term.
+
+(* Universal on wf lists: products pass through [cancel_invs] untouched and atoms
+   cancel by count, both permutation-stable (see [PreTerm.perm_cancel_invs_wf]).
+   [cancel_invs] only ever feeds [map unfold_term _], which is always wf. *)
+Global Instance cancel_invs_proper : Proper ((≡ₚ) ==> (≡ₚ)) cancel_invs.
+Proof.
+move=> ts1 ts2 H12; rewrite /cancel_invs.
+have H : PreTerm.cancel_invs (unfold_term <$> ts1)
+       ≡ₚ PreTerm.cancel_invs (unfold_term <$> ts2).
+  apply: PreTerm.perm_cancel_invs; first exact: wf_unfold_terms.
+  by rewrite H12.
+by rewrite H.
+Qed.
+
+Global Instance TExpN_proper : Proper ((=) ==> (≡ₚ) ==> (=)) TExpN.
+Proof. by move=> t _ <- ts1 ts2 ts12; apply: (TExpN_perm _ _ _ ts12). Qed.
+
+Lemma TExpC2 g t1 t2 : TExpN g [t1; t2] = TExpN g [t2; t1].
+Proof. by rewrite Permutation_swap. Qed.
+
+Global Instance term_inhabited : Inhabited term.
+Proof. exact: (populate (TInt 0)). Qed.
+
+Global Instance aenc_key_inhabited : Inhabited aenc_key :=
+  populate (AEncKey inhabitant).
+
+Global Instance sign_key_inhabited : Inhabited sign_key :=
+  populate (SignKey inhabitant).
+
+Global Instance senc_key_inhabited : Inhabited senc_key :=
+  populate (SEncKey inhabitant).
+
+Lemma subseteq_cancel_invs ts : cancel_invs ts ⊆ ts.
+Proof. apply/elem_of_subseteq => t; exact: mem_cancel_invs. Qed.
+Global Arguments subseteq_cancel_invs ts : clear implicits.
+
+Lemma TInv_neq {t} : negb (is_mul t) -> TInv t ≠ t.
+Proof. exact: TInv_Nid. Qed.
+
+Lemma elem_of_TInv_exps t1 t2 : t1 ∈ exps t2 → TInv t1 ∉ exps t2.
+Proof. exact: in_TInv_exps. Qed.
+
+Lemma elem_of_TInv_exps' t1 t2 : TInv t1 ∈ exps t2 → t1 ∉ exps t2.
+Proof. exact: in_TInv_expsV. Qed.
+
+Definition count_exp (t ts : term) : Z :=
+  (count_exp_nat t ts - count_exp_nat (TInv t) ts)%Z.
+
+Lemma count_exp_eq0 t1 t2 :
+  t1 ∉ exps t2 → TInv t1 ∉ exps t2 → count_exp t1 t2 = 0.
+Proof. by move=> ??; rewrite /count_exp !count_exp_nat_eq0. Qed.
+
+Lemma count_exp_gt0 t1 t2 : (count_exp t1 t2 > 0)%Z ↔ t1 ∈ exps t2.
+Proof.
+rewrite /count_exp; case: (decide (t1 ∈ exps t2)) => t1_t2.
+  rewrite [count_exp_nat (TInv _) _]count_exp_nat_eq0; last first.
+    exact: elem_of_TInv_exps.
+  rewrite -count_exp_nat_gt0; lia.
+rewrite count_exp_nat_eq0 //; split; first lia.
+by case/t1_t2.
+Qed.
+
+Lemma count_exp_TInv (t ts : term) : count_exp (TInv t) ts = Z.opp (count_exp t ts).
+Proof. rewrite /count_exp TInvK. lia. Qed.
+
+Lemma count_exp_TExp_eq t1 t2 :
+  negb (is_mul t1) ->
+  count_exp t1 (TExp t2 t1) = (count_exp t1 t2 + 1)%Z.
+Proof.
+move => Nm1.
+have Ht1 : t1 ≠ TInv t1 by move=> E; move: (TInv_Nid Nm1); rewrite -E.
+have E1 : count_exp_nat t1 (TExp t2 t1)
+        = S (count_exp_nat t1 t2) - (if bool_decide (TInv t1 ∈ exps t2) then 1 else 0).
+  rewrite (count_exp_nat_TExp t1 t2 t1 Nm1).
+  by rewrite (bool_decide_eq_false_2 (t1 = TInv t1) Ht1)
+             (bool_decide_eq_true_2 (t1 = t1) eq_refl).
+have E2 : count_exp_nat (TInv t1) (TExp t2 t1) = pred (count_exp_nat (TInv t1) t2).
+  rewrite (count_exp_nat_TExp (TInv t1) t2 t1 Nm1).
+  by rewrite (bool_decide_eq_true_2 (TInv t1 = TInv t1) eq_refl).
+rewrite /count_exp E1 E2; clear E1 E2.
+case_bool_decide as H.
+- have Ha : count_exp_nat t1 t2 = 0 by apply: count_exp_nat_eq0; exact: (elem_of_TInv_exps' H).
+  have Hb : count_exp_nat (TInv t1) t2 > 0 by apply/count_exp_nat_gt0.
+  rewrite Ha; lia.
+- have Hb : count_exp_nat (TInv t1) t2 = 0 by apply: count_exp_nat_eq0.
+  rewrite Hb; lia.
+Qed.
+
+Lemma count_exp_TExp_TInv t1 t2 :
+  negb (is_mul (TInv t1)) ->
+  count_exp t1 (TExp t2 (TInv t1)) = (count_exp t1 t2 - 1)%Z.
+Proof.
+move => NmI1.
+rewrite -{1}[t1]TInvK count_exp_TInv (count_exp_TExp_eq _ NmI1) count_exp_TInv.
+lia.
+Qed.
+
+Lemma count_exp_TInv_TExp t1 t2 :
+  negb (is_mul t1) ->
+  count_exp (TInv t1) (TExp t2 t1) = (count_exp (TInv t1) t2 - 1)%Z.
+Proof.
+move => Nm1.
+have h : negb (is_mul (TInv (TInv t1))) by rewrite TInvK.
+by rewrite -{2}[t1]TInvK (count_exp_TExp_TInv _ h).
+Qed.
+
+Lemma count_exp_TExp_ne t1 t2 t3 :
+  negb (is_mul t3) ->
+  t1 ≠ t3 → t1 ≠ TInv t3 → count_exp t1 (TExp t2 t3) = count_exp t1 t2.
+Proof.
+move=> Nm3 t1_t3 t1_t3V.
+have H1 : TInv t1 ≠ TInv t3 by move=> /TInv_inj E; exact: (t1_t3 E).
+have H2 : TInv t1 ≠ t3 by move=> E; apply: t1_t3V; rewrite -E TInvK.
+rewrite /count_exp (count_exp_nat_TExp t1 t2 t3 Nm3) (count_exp_nat_TExp (TInv t1) t2 t3 Nm3).
+rewrite (bool_decide_eq_false_2 (t1 = TInv t3) t1_t3V) (bool_decide_eq_false_2 (t1 = t3) t1_t3).
+by rewrite (bool_decide_eq_false_2 (TInv t1 = TInv t3) H1) (bool_decide_eq_false_2 (TInv t1 = t3) H2).
+Qed.
+
+Lemma count_exp_TExp t1 t2 t3 :
+  negb (is_mul t3) ->
+  count_exp t1 (TExp t2 t3) =
+  if decide (t1 = t3) then
+    (count_exp t1 t2 + 1)%Z
+  else if decide (t1 = TInv t3) then
+    (count_exp t1 t2 - 1)%Z
+  else count_exp t1 t2.
+Proof.
+move => Nm3.
+case: decide => [->|?]; first by rewrite count_exp_TExp_eq.
+case: decide => [->|?]; first by rewrite count_exp_TInv_TExp.
+by rewrite count_exp_TExp_ne.
+Qed.
+
+Lemma count_exp_TExpW t1 t2 t3 :
+  negb (is_mul t3) ->
+  t1 ≠ TInv t3 →
+  (count_exp t1 t2 ≤ count_exp t1 (TExp t2 t3))%Z.
+Proof.
+move=> Nm3 t1_t3; rewrite count_exp_TExp // (@decide_False _ (t1 = TInv t3)) //.
+by case: decide => ?; lia.
+Qed.
+
+Lemma not_elem_of_TInv_exps t1 t2 :
+  negb (is_mul t1) ->
+  TInv t1 ∉ exps t2 ↔ t1 ∈ exps (TExp t2 t1).
+Proof.
+move => Nm1.
+rewrite -!count_exp_gt0 count_exp_TInv count_exp_TExp_eq //; lia.
+Qed.
+
+Lemma TExpN_appC t ts1 ts2 : TExpN t (ts1 ++ ts2) = TExpN t (ts2 ++ ts1).
+Proof. exact: TExpN_catC. Qed.
+
+Inductive subterm (t : term) : term → Prop :=
+| STRefl : subterm t t
+| STPair1 t1 t2 of subterm t t1 : subterm t (TPair t1 t2)
+| STPair2 t1 t2 of subterm t t2 : subterm t (TPair t1 t2)
+| STKey kt t' of subterm t t' : subterm t (TKey kt t')
+| STSeal1 k t' of subterm t k : subterm t (TSeal k t')
+| STSeal2 k t' of subterm t t' : subterm t (TSeal k t')
+| STHash t' of subterm t t' : subterm t (THash t')
+| STInv t' of negb (is_mul t') & negb (is_inv t') & subterm t t' : subterm t (TInv t')
+| STExp1 t' ts of negb (is_exp t') & subterm t t' : subterm t (TExpN t' ts)
+| STExp2 t' t'' ts of
+    negb (is_exp t') &
+    atomic ts &
+    invs_canceled ts &
+    subterm t t'' &
+    t'' ∈ ts
+  : subterm t (TExpN t' ts)
+| STMul t'' ts of
+    wf_mul_list ts &
+    subterm t t'' &
+    t'' ∈ ts
+  : subterm t (TMulN ts).
+
+Global Instance subterm_trans : Transitive subterm.
+Proof.
+move=> t1 t2 t3 sub12 sub13; elim: t3 / sub13;
+by eauto using subterm.
+Qed.
+
+Section ValOfTerm.
+
+Fixpoint val_of_term_rec t : val :=
+  match t with
+  | TInt n =>
+    (#TOp0_tag, (#TInt_tag, #n))
+  | TPair t1 t2 =>
+    (#TOp2_tag, (#TPair_tag, val_of_term_rec t1, val_of_term_rec t2))%V
+  | TNonce l =>
+    (#TOp0_tag, (#TNonce_tag, #(nonce_loc l)))%V
+  | TKey kt t =>
+    (#TOp1_tag, ((#TKey_tag, repr kt), val_of_term_rec t))%V
+  | TSeal t1 t2 =>
+    (#TOp2_tag, (#TSeal_tag, val_of_term_rec t1, val_of_term_rec t2))%V
+  | THash t =>
+    (#TOp1_tag, ((#THash_tag, #()), val_of_term_rec t))%V
+  | TNonFree pt _ _ => val_of_pre_term pt
+  end.
+
+Definition val_of_term_aux : seal val_of_term_rec. by eexists. Qed.
+Definition val_of_term : term -> val := unseal val_of_term_aux.
+Lemma val_of_term_unseal : val_of_term = val_of_term_rec.
+Proof. exact: seal_eq. Qed.
+Coercion val_of_term : term >-> val.
+Global Instance repr_term : Repr term := val_of_term.
+
+Global Instance repr_aenc_key : Repr aenc_key := λ k : aenc_key, val_of_term (term_of_aenc_key k).
+Global Instance repr_senc_key : Repr senc_key := λ k : senc_key, val_of_term (term_of_senc_key k).
+Global Instance repr_sign_key : Repr sign_key := λ k : sign_key, val_of_term (term_of_sign_key k).
+
+Lemma val_of_pre_term_unfold t :
+  val_of_pre_term (unfold_term t) = val_of_term t.
+Proof.
+rewrite val_of_term_unseal.
+elim/term_ind': t => //=; try by move=> *; congruence.
+Qed.
+
+End ValOfTerm.
+
+Global Instance val_of_term_inj : Inj (=) (=) val_of_term.
+Proof.
+move=> t1 t2 e_t1t2; apply: unfold_term_inj.
+apply: val_of_pre_term_inj.
+by rewrite !val_of_pre_term_unfold.
+Qed.
+
+Global Instance infinite_term : Infinite term.
+Proof.
+pose int_of_term (t : term) :=
+  if t is TInt n then Some n else None.
+apply (inj_infinite TInt int_of_term).
+by move=> n; rewrite /int_of_term.
+Qed.
+
+Definition term_height t :=
+  PreTerm.height (unfold_term t).
+
+Definition nonces_of_term_def (t : term) :=
+  nonces_of_pre_term (unfold_term t).
+Arguments nonces_of_term_def /.
+Definition nonces_of_term_aux : seal nonces_of_term_def. by eexists. Qed.
+Definition nonces_of_term := unseal nonces_of_term_aux.
+Lemma nonces_of_term_unseal : nonces_of_term = nonces_of_term_def.
+Proof. exact: seal_eq. Qed.
+
+Lemma nonces_of_termE' t :
+  nonces_of_term t =
+  match t with
+  | TInt _ => ∅
+  | TPair t1 t2 => nonces_of_term t1 ∪ nonces_of_term t2
+  | TNonce l => {[l]}
+  | TKey _ t => nonces_of_term t
+  | TSeal t1 t2 => nonces_of_term t1 ∪ nonces_of_term t2
+  | THash t => nonces_of_term t
+  | TNonFree pt _ _ => nonces_of_pre_term pt
+  end.
+Proof.
+by rewrite nonces_of_term_unseal; case: t => //=.
+Qed.
+
+Lemma nonces_of_term_fold pt :
+  PreTerm.wf pt -> nonces_of_term (fold_term pt) = nonces_of_pre_term pt.
+Proof. move => wf. by rewrite nonces_of_term_unseal /nonces_of_term_def (@fold_termK pt wf). Qed.
+
+Lemma nonces_of_pre_term_factors e :
+  nonces_of_pre_term e = ⋃ map nonces_of_pre_term (PreTerm.factors e).
+Proof. by case: e => [o|o1 e1|o2 e1 e2|es] //=; rewrite union_empty_r_L. Qed.
+
+Lemma nonces_of_pre_term_inv_aux x :
+  nonces_of_pre_term (PreTerm.inv_aux x) = nonces_of_pre_term x.
+Proof. by case: x => [o|[kt||] e|o e1 e2|es] //=. Qed.
+
+(* Local bridge: [merge_sort] only permutes, and [⋃ ∘ map f] is
+   permutation-invariant, so sorting the list before mapping is transparent. *)
+Lemma union_list_map_merge_sort {A X} `{Countable X} (f : A → gset X)
+  (R : relation A) `{!RelDecision R} l :
+  ⋃ map f (merge_sort R l) = ⋃ map f l.
+Proof.
+apply: union_list_permutation_proper_L; apply: Permutation_map.
+exact: (merge_sort_Permutation R l).
+Qed.
+
+(* [inv] distributes [inv] over the factors and re-multiplies; [inv] preserves
+   nonces, and (for wf [pt]) no cancellation occurs, so nonces are preserved. *)
+Lemma nonces_of_pre_term_inv pt :
+  PreTerm.wf pt ->
+  nonces_of_pre_term (PreTerm.inv pt) = nonces_of_pre_term pt.
+Proof.
+move => wf.
+rewrite (PreTerm.inv_factors pt wf) (nonces_of_pre_term_factors pt).
+set F := PreTerm.factors pt.
+have wfF : Forall PreTerm.wf F := PreTerm.wf_factors pt wf.
+have NmF : Forall (fun pt => negb (PreTerm.is_mul pt)) F := PreTerm.Nmul_factors pt wf.
+have cancF : PreTerm.invs_canceled F := PreTerm.invs_canceled_factors pt wf.
+have wfMI : Forall PreTerm.wf (PreTerm.inv_aux <$> F).
+  apply/Forall_fmap; apply/Forall_forall => x xF.
+  apply: PreTerm.wf_inv_aux; [exact: (Forall_mem wfF xF) | exact: (Forall_mem NmF xF)].
+have NmMI : Forall (fun pt => negb (PreTerm.is_mul pt)) (PreTerm.inv_aux <$> F).
+  apply/Forall_fmap; apply/Forall_forall => x xF.
+  apply: PreTerm.is_mul_inv_aux; exact: (Forall_mem wfF xF).
+have cancMI : PreTerm.invs_canceled (PreTerm.inv_aux <$> F).
+  exact: PreTerm.invs_canceled_map_inv F wfF cancF.
+rewrite (nonces_of_pre_term_factors (PreTerm.mul (PreTerm.inv_aux <$> F))).
+rewrite (PreTerm.factors_mul (PreTerm.inv_aux <$> F) wfMI).
+rewrite (PreTerm.flatten_factors_Nmul_id (PreTerm.inv_aux <$> F) NmMI).
+rewrite (PreTerm.cancel_invs_canceled (PreTerm.inv_aux <$> F) NmMI cancMI).
+rewrite union_list_map_merge_sort.
+rewrite /F; elim: (PreTerm.factors pt) => [//|x fs IH] /=.
+by rewrite nonces_of_pre_term_inv_aux IH.
+Qed.
+
+Lemma nonces_of_term_TInv t : nonces_of_term (TInv t) = nonces_of_term t.
+Proof.
+rewrite !nonces_of_term_unseal /nonces_of_term_def unfold_TInv.
+exact: nonces_of_pre_term_inv (wf_unfold_term t).
+Qed.
+
+(* Elementwise: folding the inverse of a well-formed atomic factor is [TInv] of
+   the folded factor.  Stated as a standalone lemma to keep [fmap]'s typeclass
+   instance resolved (a [have] with [<$>] in its type spuriously generalises it). *)
+Lemma fmap_fold_inv_aux G :
+  Forall PreTerm.wf G ->
+  Forall (fun pt => negb (PreTerm.is_mul pt)) G ->
+  fold_term <$> (PreTerm.inv_aux <$> G) = TInv <$> (fold_term <$> G).
+Proof.
+elim: G => [//|x fs IH] /Forall_cons [Wx wfs] /Forall_cons [Nmx Nms].
+rewrite !fmap_cons (IH wfs Nms); congr cons.
+apply: unfold_term_inj.
+by rewrite unfold_TInv (fold_termK x Wx)
+           (fold_termK (PreTerm.inv_aux x) (PreTerm.wf_inv_aux x Wx Nmx))
+           (PreTerm.inv_Nmul x Nmx).
+Qed.
+
+(* [TInv] distributes over products: the canonical factor list of [TInv t] is
+   a permutation of the inverses of the factors of [t].  Used to prove
+   [public (TInv t) ⊣⊢ public t] for products by reducing to the factors. *)
+Lemma tfactors_TInv t : tfactors (TInv t) ≡ₚ map TInv (tfactors t).
+Proof.
+rewrite /tfactors unfold_TInv (PreTerm.inv_factors (unfold_term t) (wf_unfold_term t)).
+set F := PreTerm.factors (unfold_term t).
+have wfF : Forall PreTerm.wf F := PreTerm.wf_factors _ (wf_unfold_term t).
+have NmF : Forall (fun pt => negb (PreTerm.is_mul pt)) F := PreTerm.Nmul_factors _ (wf_unfold_term t).
+have cancF : PreTerm.invs_canceled F := PreTerm.invs_canceled_factors _ (wf_unfold_term t).
+have wfMI : Forall PreTerm.wf (PreTerm.inv_aux <$> F).
+  apply/Forall_fmap; apply/Forall_forall => x xF.
+  apply: PreTerm.wf_inv_aux; [exact: (Forall_mem wfF xF) | exact: (Forall_mem NmF xF)].
+have NmMI : Forall (fun pt => negb (PreTerm.is_mul pt)) (PreTerm.inv_aux <$> F).
+  apply/Forall_fmap; apply/Forall_forall => x xF.
+  apply: PreTerm.is_mul_inv_aux; exact: (Forall_mem wfF xF).
+have cancMI : PreTerm.invs_canceled (PreTerm.inv_aux <$> F).
+  exact: PreTerm.invs_canceled_map_inv F wfF cancF.
+rewrite (PreTerm.factors_mul (PreTerm.inv_aux <$> F) wfMI).
+rewrite (PreTerm.flatten_factors_Nmul_id (PreTerm.inv_aux <$> F) NmMI).
+rewrite (PreTerm.cancel_invs_canceled (PreTerm.inv_aux <$> F) NmMI cancMI).
+rewrite (merge_sort_Permutation pt_order (PreTerm.inv_aux <$> F)).
+by rewrite (fmap_fold_inv_aux wfF NmF).
+Qed.
+
+Lemma nonces_of_pre_term_base_expo pt :
+  nonces_of_pre_term pt =
+  nonces_of_pre_term (PreTerm.base pt) ∪ nonces_of_pre_term (PreTerm.expo pt).
+Proof. by case: pt => [o|o1 e1|[||] e1 e2|es] //=; rewrite union_empty_r_L. Qed.
+
+Lemma nonces_of_term_base_exps t :
+  nonces_of_term t = nonces_of_term (base t) ∪ ⋃ map nonces_of_term (exps t).
+Proof.
+transitivity (nonces_of_pre_term (PreTerm.base (unfold_term t)) ∪
+              ⋃ map nonces_of_pre_term (PreTerm.exps (unfold_term t))).
+  rewrite {1}nonces_of_term_unseal /nonces_of_term_def.
+  rewrite (nonces_of_pre_term_base_expo (unfold_term t)).
+  by rewrite (nonces_of_pre_term_factors (PreTerm.expo (unfold_term t))).
+congr (_ ∪ _).
+  by rewrite /base (nonces_of_term_fold (PreTerm.wf_base _ (wf_unfold_term t))).
+rewrite /exps.
+have wfs : Forall PreTerm.wf (PreTerm.exps (unfold_term t)) := PreTerm.wf_exps _ (wf_unfold_term t).
+elim: (PreTerm.exps (unfold_term t)) wfs => [//|pt pts IH] /Forall_cons [wpt wpts] /=.
+by rewrite (nonces_of_term_fold wpt) (IH wpts).
+Qed.
+
+Lemma nonces_of_term_TExpN t ts :
+  negb (is_exp t) -> atomic ts ->
+  nonces_of_term (TExpN t ts) = nonces_of_term t ∪ ⋃ map nonces_of_term (cancel_invs ts).
+Proof.
+move => tNexp atom.
+have nexp : negb (PreTerm.is_exp (unfold_term t)).
+  by move: tNexp; rewrite is_exp_unfold.
+have bt : base t = t by rewrite /base (PreTerm.base_expN _ nexp) unfold_termK.
+have et : exps t = [] by rewrite /exps (PreTerm.exps_expN _ nexp).
+rewrite (nonces_of_term_base_exps (TExpN t ts)) base_TExpN bt.
+congr (_ ∪ _).
+by rewrite (exps_TExpN_sort t ts atom) et app_nil_l union_list_map_merge_sort.
+Qed.
+
+Lemma nonces_flatten_factors us :
+  ⋃ map nonces_of_pre_term (concat (PreTerm.factors <$> us)) =
+  ⋃ map nonces_of_pre_term us.
+Proof.
+elim: us => [|u us IH] //=.
+by rewrite map_app union_list_app_L -(nonces_of_pre_term_factors u) IH.
+Qed.
+
+(* [PreTerm.mul] cancels/sorts/flattens its argument, so its nonces are a subset
+   of the union of the factors' nonces — no atomicity needed. *)
+Lemma nonces_of_pre_term_mul_sub us :
+  nonces_of_pre_term (PreTerm.mul us) ⊆ ⋃ map nonces_of_pre_term us.
+Proof.
+rewrite /PreTerm.mul.
+set M := concat (PreTerm.factors <$> us).
+rewrite (_ : nonces_of_pre_term _ =
+             ⋃ map nonces_of_pre_term
+                 (merge_sort pt_order (PreTerm.cancel_invs M))); last first.
+  by case: (merge_sort pt_order (PreTerm.cancel_invs M)) => [|t [|t' l]] //=;
+     rewrite union_empty_r_L.
+rewrite union_list_map_merge_sort.
+have HM : ⋃ map nonces_of_pre_term M = ⋃ map nonces_of_pre_term us
+  by rewrite /M nonces_flatten_factors.
+rewrite -HM.
+move => a /elem_of_union_list [X [/list_elem_of_fmap [x [-> xL]] aX]].
+apply/elem_of_union_list; exists (nonces_of_pre_term x); split => //.
+apply/list_elem_of_fmap; exists x; split => //.
+exact: (PreTerm.mem_cancel_invs M x xL).
+Qed.
+
+(* [PreTerm.exp] folds the new exponent into the base and cancels, so nonces are a
+   subset of [nonces base ∪ nonces exponent] — no atomicity needed. *)
+Lemma nonces_of_pre_term_exp_sub b e :
+  nonces_of_pre_term (PreTerm.exp b e) ⊆ nonces_of_pre_term b ∪ nonces_of_pre_term e.
+Proof.
+rewrite /PreTerm.exp; cbv zeta.
+have Hbe := nonces_of_pre_term_base_expo b.
+case: (bool_decide (PreTerm.mul [PreTerm.expo b; e] = PreTerm.PTMul [])).
+- set_solver.
+- have Hmul := @nonces_of_pre_term_mul_sub [PreTerm.expo b; e].
+  move: Hmul => /=; set_solver.
+Qed.
+
+(* The atomicity hypothesis is not needed: [TExpN t ts = TExp t (TMulN ts)], and the
+   nonces of both [exp] and [mul] are subsets of their parts regardless of atomicity. *)
+Lemma nonces_of_term_TExpN_subseteq t ts :
+  nonces_of_term (TExpN t ts) ⊆ nonces_of_term t ∪ ⋃ map nonces_of_term ts.
+Proof.
+have Hts : ⋃ map nonces_of_term ts = ⋃ map nonces_of_pre_term (map unfold_term ts).
+  congr union_list. elim: ts => [|t' ts IH] //=.
+  by rewrite IH nonces_of_term_unseal /nonces_of_term_def.
+rewrite Hts !nonces_of_term_unseal /nonces_of_term_def.
+have -> : unfold_term (TExpN t ts) =
+          PreTerm.exp (unfold_term t) (PreTerm.mul (map unfold_term ts)).
+  by rewrite /TExpN unfold_TExp unfold_TMulN.
+etrans; first exact: (@nonces_of_pre_term_exp_sub (unfold_term t)
+                        (PreTerm.mul (map unfold_term ts))).
+have Hmul := @nonces_of_pre_term_mul_sub (map unfold_term ts).
+set_solver.
+Qed.
+Global Arguments nonces_of_term_TExpN_subseteq t ts : clear implicits.
+
+Lemma nonces_of_term_TMulN ts :
+  wf_mul_list ts ->
+  nonces_of_term (TMulN ts) = ⋃ map nonces_of_term ts.
+Proof.
+move => wf; have wfU := wf_mul_list_unfold ts wf.
+have e : TMulN ts = fold_term (PreTerm.PTMul (map unfold_term ts)).
+  apply: unfold_term_inj; rewrite unfold_TMulN (@fold_termK _ wfU).
+  exact: (PreTerm.mul_factors _ wfU).
+rewrite {1}e (nonces_of_term_fold wfU) /=.
+elim: ts {wf wfU e} => [//|t' ts' IH] /=.
+rewrite -IH; congr (_ ∪ _).
+by rewrite nonces_of_term_unseal.
+Qed.
+
+Lemma nonces_of_term_tfactors t :
+  nonces_of_term t = ⋃ map nonces_of_term (tfactors t).
+Proof.
+rewrite nonces_of_term_unseal /nonces_of_term_def
+  (nonces_of_pre_term_factors (unfold_term t)) /tfactors.
+congr union_list.
+elim: (PreTerm.factors (unfold_term t)) (PreTerm.wf_factors _ (wf_unfold_term t))
+  => [//|pt pts IH] /Forall_cons [wpt wpts] /=.
+by rewrite (fold_termK pt wpt) (IH wpts).
+Qed.
+
+Definition nonces_of_termE :=
+  (nonces_of_term_TInv, nonces_of_term_TExpN, nonces_of_term_TMulN, nonces_of_termE').
+
+Fixpoint ssubterms_pre_def (t : PreTerm.pre_term) : gset term :=
+  let subterms_pre_def (t : PreTerm.pre_term) := {[fold_term t]} ∪ ssubterms_pre_def t in
+  match t with
+  | PreTerm.PT0 (O0Int _) => ∅
+  | PreTerm.PT2 O2Pair t1 t2 => subterms_pre_def t1 ∪ subterms_pre_def t2
+  | PreTerm.PT0 (O0Nonce _) => ∅
+  | PreTerm.PT1 (O1Key _) t => subterms_pre_def t
+  | PreTerm.PT2 O2Seal t1 t2 => subterms_pre_def t1 ∪ subterms_pre_def t2
+  | PreTerm.PT1 O1Hash t => subterms_pre_def t
+  | PreTerm.PT1 O1Inv t => subterms_pre_def t
+  | PreTerm.PTExp b (PreTerm.PTMul us) =>
+    subterms_pre_def b ∪ ⋃ map subterms_pre_def us
+  | PreTerm.PTExp b e => subterms_pre_def b ∪ subterms_pre_def e
+  | PreTerm.PTMul ts => ⋃ map subterms_pre_def ts
+  end.
+
+Definition subterms_def t := {[t]} ∪ ssubterms_pre_def (unfold_term t).
+Arguments subterms_def /.
+Definition subterms_aux : seal subterms_def. by eexists. Qed.
+Definition subterms := unseal subterms_aux.
+Lemma subterms_unseal : subterms = subterms_def.
+Proof. exact: seal_eq. Qed.
+
+Definition subterms_pre pt := {[fold_term pt]} ∪ ssubterms_pre_def pt.
+
+Lemma subterms_preE pt :
+  subterms_pre pt =
+  {[fold_term pt]} ∪
+  match pt with
+  | PreTerm.PT0 _ => ∅
+  | PreTerm.PT1 (O1Key _) t => subterms_pre t
+  | PreTerm.PT1 O1Hash t => subterms_pre t
+  | PreTerm.PT1 O1Inv t => subterms_pre t
+  | PreTerm.PT2 O2Pair t1 t2 => subterms_pre t1 ∪ subterms_pre t2
+  | PreTerm.PT2 O2Seal t1 t2 => subterms_pre t1 ∪ subterms_pre t2
+  | PreTerm.PTExp b e => subterms_pre b ∪ ⋃ map subterms_pre (PreTerm.factors e)
+  | PreTerm.PTMul ts => ⋃ map subterms_pre ts
+  end.
+Proof.
+rewrite /subterms_pre; case: pt => [o|o e|[||] e1 e2|es] //=.
+- by case: o.
+- case: e2 => //= *; set_solver.
+Qed.
+
+Lemma subterms_fold pt :
+  PreTerm.wf pt -> subterms (fold_term pt) = subterms_pre pt.
+Proof. move => wf; by rewrite subterms_unseal /subterms_def /subterms_pre (@fold_termK pt wf). Qed.
+
+Lemma subterms_via_pre t : subterms t = subterms_pre (unfold_term t).
+Proof. by rewrite subterms_unseal /subterms_def /subterms_pre unfold_termK. Qed.
+
+Lemma subterms_pre_base_exps pt :
+  subterms_pre pt =
+  {[fold_term pt]} ∪ subterms_pre (PreTerm.base pt) ∪ ⋃ map subterms_pre (PreTerm.exps pt).
+Proof.
+case E: (PreTerm.is_exp pt).
+- case: pt E => [o|o e|[||] e1 e2|es] //= E; rewrite subterms_preE /=; set_solver.
+- have Nxp : negb (PreTerm.is_exp pt) by rewrite E.
+  rewrite (PreTerm.base_expN pt Nxp) (PreTerm.exps_expN pt Nxp) /=.
+  rewrite /subterms_pre; set_solver.
+Qed.
+
+Lemma subterms_base_exps t :
+  subterms t = {[t]} ∪ subterms (base t) ∪ ⋃ map subterms (exps t).
+Proof.
+have hb : subterms_pre (PreTerm.base (unfold_term t)) = subterms (base t).
+  by rewrite /base (subterms_fold (PreTerm.wf_base _ (wf_unfold_term t))).
+have he : ⋃ map subterms_pre (PreTerm.exps (unfold_term t)) = ⋃ map subterms (exps t).
+  rewrite /exps.
+  have wfs : Forall PreTerm.wf (PreTerm.exps (unfold_term t)) := PreTerm.wf_exps _ (wf_unfold_term t).
+  elim: (PreTerm.exps (unfold_term t)) wfs => [//|pt pts IH] /Forall_cons [wpt wpts] /=.
+  by rewrite (subterms_fold wpt) (IH wpts).
+by rewrite (subterms_via_pre t) (subterms_pre_base_exps (unfold_term t)) unfold_termK hb he.
+Qed.
+
+Lemma subtermsE' t :
+  subterms t =
+  {[t]} ∪
+  match t with
+  | TInt _ => ∅
+  | TPair t1 t2 => subterms t1 ∪ subterms t2
+  | TNonce _ => ∅
+  | TKey _ t => subterms t
+  | TSeal t1 t2 => subterms t1 ∪ subterms t2
+  | THash t => subterms t
+  | TNonFree pt _ _ => ssubterms_pre_def pt
+  end.
+Proof.
+rewrite subterms_unseal /=.
+case: t =>> //=; try by rewrite ?unfold_termK.
+Qed.
+
+Lemma subterms_TInv t :
+  negb (is_mul t) -> negb (is_inv t) ->
+  subterms (TInv t) = {[TInv t]} ∪ subterms t.
+Proof.
+move => Nm Ni.
+have Ni' : negb (PreTerm.is_inv (unfold_term t)) by rewrite -is_inv_unfold.
+rewrite subterms_unseal /subterms_def.
+by rewrite (unfold_TInv_Nmul Nm) (PreTerm.inv_invN _ Ni') /= unfold_termK.
+Qed.
+
+Lemma subterms_TExpN t ts :
+  negb (is_exp t) -> atomic ts ->
+  subterms (TExpN t ts) = {[TExpN t ts]} ∪ subterms t ∪ ⋃ map subterms (cancel_invs ts).
+Proof.
+move => tNexp atom.
+have nexp : negb (PreTerm.is_exp (unfold_term t)).
+  by move: tNexp; rewrite is_exp_unfold.
+have bt : base t = t by rewrite /base (PreTerm.base_expN _ nexp) unfold_termK.
+have et : exps t = [] by rewrite /exps (PreTerm.exps_expN _ nexp).
+rewrite (subterms_base_exps (TExpN t ts)) base_TExpN bt.
+by rewrite (exps_TExpN_sort t ts atom) et app_nil_l union_list_map_merge_sort.
+Qed.
+
+Lemma subterms_TMulN ts :
+  wf_mul_list ts ->
+  subterms (TMulN ts) = {[TMulN ts]} ∪ ⋃ map subterms ts.
+Proof.
+move => wf; have wfU := wf_mul_list_unfold ts wf.
+have e : TMulN ts = fold_term (PreTerm.PTMul (map unfold_term ts)).
+  apply: unfold_term_inj; rewrite unfold_TMulN (@fold_termK _ wfU).
+  exact: (PreTerm.mul_factors _ wfU).
+rewrite {1}e (subterms_fold wfU) subterms_preE -e /=.
+congr (_ ∪ _).
+elim: ts {wf wfU e} => [//|t' ts' IH] /=.
+rewrite -IH; congr (_ ∪ _).
+by rewrite subterms_via_pre.
+Qed.
+
+Lemma subterms_nonce t : is_nonce t → subterms t = {[t]}.
+Proof.
+by case: t => //= ? _; rewrite subtermsE' right_id_L.
+Qed.
+
+Definition subtermsE := (subterms_TInv, subterms_TExpN, subterms_TMulN, subtermsE').
+
+Ltac solve_subtermsP :=
+  intros;
+  repeat match goal with
+  | H : context[subterms (?X ?Y)] |- _ =>
+      rewrite [subterms (X Y)]subtermsE /= in H
+  | H : _ ∈ {[_]} |- _ =>
+      rewrite elem_of_singleton in H;
+      rewrite {}H
+  | H : _ ∈ _ ∪ _ |- _ =>
+      rewrite elem_of_union in H;
+      destruct H
+  | H : _ ∈ ∅ |- _ =>
+      rewrite elem_of_empty in H;
+      destruct H
+  | H1 : ?P, H2 : ?P -> ?Q |- _ =>
+      move/(_ H1) in H2
+  end;
+  eauto using subterm.
+
+Lemma subtermsP t1 t2 : subterm t1 t2 ↔ t1 ∈ subterms t2.
+Proof.
+split.
+- elim: t2 /; try by intros; rewrite subtermsE //; set_solver.
+  + move => t' ts Nexp sub IH.
+    have bt' : base t' = t'.
+      rewrite /base; move: Nexp; rewrite is_exp_unfold => n.
+      by rewrite (PreTerm.base_expN _ n) unfold_termK.
+    rewrite (subterms_base_exps (TExpN t' ts)) base_TExpN bt'; set_solver.
+  + move => t' t'' ts Nexp atom canc sub IH t''_ts.
+    rewrite (subterms_TExpN Nexp atom).
+    rewrite (cancel_invs_canceled ts atom canc) !elem_of_union; right.
+    rewrite elem_of_union_list; exists (subterms t''); split => //.
+    by rewrite list_elem_of_fmap; exists t''; split.
+  + move => t'' ts wf sub IH t''_ts.
+    rewrite (subterms_TMulN wf) elem_of_union; right.
+    rewrite elem_of_union_list; exists (subterms t''); split => //.
+    by rewrite list_elem_of_fmap; exists t''; split.
+- elim: t2; try by solve_subtermsP.
+  + move => t IHt Nexp ts IHts atom tsN0 sort canc.
+    rewrite subtermsE //.
+    rewrite (cancel_invs_canceled ts atom canc).
+    rewrite !elem_of_union elem_of_union_list elem_of_singleton.
+    case => [[-> | /IHt sub] | [X [/list_elem_of_fmap [t' [-> t'_ts]] t1_t']]].
+    * exact: STRefl.
+    * apply: STExp1; [exact: Nexp|exact: sub].
+    * have sub' : subterm t1 t'.
+        move: IHts t'_ts t1_t'; elim: (ts) => /= [_ /elem_of_nil //|t0 ts0 IH0 [IH1 IHrest]].
+        rewrite elem_of_cons; case => [-> //|/(IH0 IHrest)] // h ?; exact: h.
+      apply: (STExp2 Nexp atom canc sub' t'_ts).
+  + move => ts IHts atom sort canc szN1.
+    have wf : wf_mul_list ts := conj atom (conj sort (conj canc szN1)).
+    rewrite (subterms_TMulN wf).
+    rewrite elem_of_union elem_of_union_list elem_of_singleton.
+    case => [-> | [X [/list_elem_of_fmap [t' [-> t'_ts]] t1_t']]].
+    * exact: STRefl.
+    * have sub' : subterm t1 t'.
+        move: IHts t'_ts t1_t'; elim: (ts) => /= [_ /elem_of_nil //|t0 ts0 IH0 [IH1 IHrest]].
+        rewrite elem_of_cons; case => [-> //|/(IH0 IHrest)] // h ?; exact: h.
+      apply: (STMul wf sub' t'_ts).
+Qed.
+
+Ltac solve_nonces_of_termP :=
+  intros;
+  repeat match goal with
+  | H : context[nonces_of_term (?X ?Y)] |- _ =>
+      rewrite [nonces_of_term (X Y)]nonces_of_termE /= in H
+  | H : _ ∈ {[_]} |- _ =>
+      rewrite elem_of_singleton in H;
+      rewrite {}H
+  | H : _ ∈ _ ∪ _ |- _ =>
+      rewrite elem_of_union in H;
+      destruct H
+  | H : _ ∈ ∅ |- _ =>
+      rewrite elem_of_empty in H;
+      destruct H
+  | H1 : ?P, H2 : ?P -> ?Q |- _ =>
+      move/(_ H1) in H2
+  end;
+  eauto using subterm.
+
+Lemma nonces_of_termP (a : nonce) t : subterm (TNonce a) t ↔ a ∈ nonces_of_term t.
+Proof.
+split.
+- elim: t /; try by intros; rewrite nonces_of_termE; set_solver.
+  + move => t' ts Nexp sub IH.
+    have bt' : base t' = t'.
+      rewrite /base; move: Nexp; rewrite is_exp_unfold => n.
+      by rewrite (PreTerm.base_expN _ n) unfold_termK.
+    rewrite (nonces_of_term_base_exps (TExpN t' ts)) base_TExpN bt'; set_solver.
+  + move => t' t'' ts Nexp atom canc sub IH t''_ts.
+    rewrite (nonces_of_term_TExpN Nexp atom).
+    rewrite (cancel_invs_canceled ts atom canc) elem_of_union; right.
+    rewrite elem_of_union_list; exists (nonces_of_term t''); split => //.
+    by rewrite list_elem_of_fmap; exists t''; split.
+  + move => t'' ts wf sub IH t''_ts.
+    rewrite (nonces_of_term_TMulN wf) elem_of_union_list.
+    exists (nonces_of_term t''); split => //.
+    by rewrite list_elem_of_fmap; exists t''; split.
+- elim: t; try by solve_nonces_of_termP.
+  + move => t IHt Nexp ts IHts atom tsN0 sort canc.
+    rewrite nonces_of_termE //.
+    rewrite (cancel_invs_canceled ts atom canc) elem_of_union elem_of_union_list.
+    case => [/IHt sub | [X [/list_elem_of_fmap [t' [-> t'_ts]] a_t']]].
+    * apply: STExp1; [exact: Nexp|exact: sub].
+    * have sub' : subterm (TNonce a) t'.
+        move: IHts t'_ts a_t'; elim: (ts) => /= [_ /elem_of_nil //|t0 ts0 IH0 [IH1 IHrest]].
+        rewrite elem_of_cons; case => [-> //|/(IH0 IHrest)] // h ?; exact: h.
+      apply: (STExp2 Nexp atom canc sub' t'_ts).
+  + move => ts IHts atom sort canc szN1.
+    have wf : wf_mul_list ts := conj atom (conj sort (conj canc szN1)).
+    rewrite (nonces_of_term_TMulN wf) elem_of_union_list.
+    case => [X [/list_elem_of_fmap [t' [-> t'_ts]] a_t']].
+    have sub' : subterm (TNonce a) t'.
+      move: IHts t'_ts a_t'; elim: (ts) => /= [_ /elem_of_nil //|t0 ts0 IH0 [IH1 IHrest]].
+      rewrite elem_of_cons; case => [-> //|/(IH0 IHrest)] // h ?; exact: h.
+    apply: (STMul wf sub' t'_ts).
+Qed.
+
+Lemma subterm_nonces_of_term t1 t2 :
+  subterm t1 t2 → nonces_of_term t1 ⊆ nonces_of_term t2.
+Proof.
+elim: t2 / => //; try by intros; rewrite [nonces_of_term (_ _)]nonces_of_termE; set_solver.
+- move => t' ts Nexp sub IH.
+  have bt' : base t' = t'.
+    rewrite /base; move: Nexp; rewrite is_exp_unfold => n.
+    by rewrite (PreTerm.base_expN _ n) unfold_termK.
+  rewrite (nonces_of_term_base_exps (TExpN t' ts)) base_TExpN bt'; set_solver.
+- move => t' t'' ts Nexp atom canc sub IH t''_ts.
+  rewrite (nonces_of_term_TExpN Nexp atom).
+  rewrite (cancel_invs_canceled ts atom canc).
+  have sub2 : nonces_of_term t'' ⊆ ⋃ map nonces_of_term ts.
+    move => x x_t''; rewrite elem_of_union_list; exists (nonces_of_term t''); split => //.
+    by rewrite list_elem_of_fmap; exists t''; split.
+  set_solver.
+- move => t'' ts wf sub IH t''_ts.
+  rewrite (nonces_of_term_TMulN wf).
+  have sub2 : nonces_of_term t'' ⊆ ⋃ map nonces_of_term ts.
+    move => x x_t''; rewrite elem_of_union_list; exists (nonces_of_term t''); split => //.
+    by rewrite list_elem_of_fmap; exists t''; split.
+  set_solver.
+Qed.
+
+Definition Tag_def (N : namespace) :=
+  TInt (Zpos (encode N)).
+Definition Tag_aux : seal Tag_def. by eexists. Qed.
+Definition Tag := unseal Tag_aux.
+Lemma Tag_unseal : Tag = Tag_def. Proof. exact: seal_eq. Qed.
+
+Global Instance Tag_inj : Inj (=) (=) Tag.
+Proof. by rewrite Tag_unseal => ?? [] /(inj _ _ _). Qed.
+
+Module Spec.
+
+Implicit Types N : term.
+
+Definition is_seal_key k :=
+  match k with
+  | TKey AEnc _ | TKey Sign _ | TKey SEnc _ => true
+  | _ => false
+  end.
+
+Definition public_key_type kt :=
+  match kt with
+  | AEnc | Verify => true
+  | _ => false
+  end.
+
+Definition skey t :=
+  match t with
+  | TKey AEnc t => TKey ADec t
+  | TKey Verify t => TKey Sign t
+  | _ => t
+  end.
+
+Definition pkey t :=
+  match t with
+  | TKey ADec t => TKey AEnc t
+  | TKey Sign t => TKey Verify t
+  | _ => t
+  end.
+
+Lemma aenc_pkey_inj (sk1 sk2 : aenc_key) :
+  pkey sk1 = pkey sk2 → sk1 = sk2.
+Proof. by rewrite keysE; case: sk1 sk2 => [?] [?] [->]. Qed.
+
+Lemma sign_pkey_inj (sk1 sk2 : sign_key) :
+  pkey sk1 = pkey sk2 → sk1 = sk2.
+Proof. by rewrite keysE; case: sk1 sk2 => [?] [?] [->]. Qed.
+
+Lemma senc_pkey_inj (sk1 sk2 : senc_key) :
+  pkey sk1 = pkey sk2 → sk1 = sk2.
+Proof. by rewrite keysE; case: sk1 sk2 => [?] [?] [->]. Qed.
+
+Definition tag_def N (t : term) :=
+  TPair N t.
+Definition tag_aux : seal tag_def. by eexists. Qed.
+Definition tag := unseal tag_aux.
+Lemma tag_unseal : tag = tag_def. Proof. exact: seal_eq. Qed.
+
+Lemma is_nonce_tag N t : is_nonce (tag N t) = false.
+Proof. by rewrite tag_unseal. Qed.
+
+Lemma is_exp_tag N t : is_exp (tag N t) = false.
+Proof. by rewrite tag_unseal. Qed.
+
+Definition untag_def N (t : term) :=
+  match t with
+  | TPair N' t =>
+    if decide (N = N') then Some t else None
+  | _ => None
+  end.
+Definition untag_aux : seal untag_def. by eexists. Qed.
+Definition untag := unseal untag_aux.
+Lemma untag_unseal : untag = untag_def. Proof. exact: seal_eq. Qed.
+
+Lemma tagK N t : untag N (tag N t) = Some t.
+Proof.
+rewrite untag_unseal tag_unseal /untag_def /tag_def /=.
+by rewrite decide_True_pi.
+Qed.
+
+#[global]
+Instance tag_inj : Inj2 (=) (=) (=) tag.
+Proof.
+rewrite tag_unseal /tag_def => c1 t1 c2 t2 [] e ->.
+split=> //; by apply: inj e.
+Qed.
+
+Lemma untagK N t1 t2 :
+  untag N t1 = Some t2 ->
+  t1 = tag N t2.
+Proof.
+rewrite untag_unseal tag_unseal /=.
+case: t1=> [] // N' t1 /=.
+by case: decide => // <- [<-].
+Qed.
+
+Lemma untag_tag_ne N1 N2 t :
+  N1 ≠ N2 →
+  Spec.untag N1 (Spec.tag N2 t) = None.
+Proof.
+move=> neq; rewrite Spec.untag_unseal Spec.tag_unseal /=.
+rewrite decide_False //.
+Qed.
+
+Variant untag_spec N t : option term → Type :=
+| UntagSome t' of t = Spec.tag N t' : untag_spec N t (Some t')
+| UntagNone of (∀ t', t ≠ Spec.tag N t') : untag_spec N t None.
+
+Lemma untagP N t : untag_spec N t (Spec.untag N t).
+Proof.
+case e: (Spec.untag N t) => [t'|]; constructor.
+- by rewrite (Spec.untagK e).
+- move=> t' e'; by rewrite e' Spec.tagK in e.
+Qed.
+
+Definition to_int t :=
+  if t is TInt n then Some n else None.
+
+Variant to_int_spec t : option Z → Type :=
+| AsIntSome n of t = TInt n : to_int_spec t (Some n)
+| AsIntNone of (∀ n, t ≠ TInt n) : to_int_spec t None.
+
+Lemma to_intP t : to_int_spec t (Spec.to_int t).
+Proof. by case: t => *; constructor; congruence. Qed.
+
+Definition untuple t :=
+  match t with
+  | TPair t1 t2 => Some (t1, t2)
+  | _ => None
+  end.
+
+Fixpoint proj t n {struct t} :=
+  match t, n with
+  | TPair t _, 0 => Some t
+  | TPair _ t, S n => proj t n
+  | _, _ => None
+  end.
+
+Definition to_key k : option (key_type * term) :=
+  match k with
+  | TKey kt t => Some (kt, t)
+  | _ => None
+  end.
+
+Definition open_key k : option term :=
+  match to_key k with
+  | Some (kt, t) =>
+      match kt with
+      | AEnc => Some (TKey ADec t)
+      | Sign => Some (TKey Verify t)
+      | SEnc => Some (TKey SEnc t)
+      | _ => None
+      end
+  | _ => None
+  end.
+
+Lemma open_key_aenc (sk : aenc_key) :
+  open_key (Spec.pkey sk) = @Some term sk.
+Proof. by rewrite keysE. Qed.
+
+Lemma open_key_sign (sk : sign_key) :
+  open_key sk = Some (Spec.pkey sk).
+Proof. by rewrite keysE. Qed.
+
+Lemma open_key_senc (sk : senc_key) :
+  open_key sk = @Some term sk.
+Proof. by rewrite keysE. Qed.
+
+Lemma open_key_aencK pk (sk : aenc_key) :
+  open_key pk = @Some term sk → pk = pkey sk.
+Proof.
+rewrite keysE; case: sk => seed /=.
+by case: pk => //= - [] // ?; case=> ->.
+Qed.
+
+Lemma open_key_signK k (sk : sign_key) :
+  open_key k = Some (Spec.pkey sk) → k = sk.
+Proof.
+rewrite keysE; case: sk => seed /=.
+by case: k => //= - [] // ?; case=> ->.
+Qed.
+
+Lemma open_key_sencK k' (k : senc_key) :
+  open_key k' = @Some term k → k' = k.
+Proof.
+rewrite keysE; case: k => seed /=.
+by case: k' => //= - [] // ?; case=> ->.
+Qed.
+
+Lemma open_key_tsize t1 t2 : open_key t1 = Some t2 → tsize t2 = tsize t1.
+Proof.
+by case: t1 => // - [] //= t [<-]; rewrite tsizeE.
+Qed.
+
+Definition open k t : option term :=
+  match t with
+  | TSeal k_t t =>
+    if decide (open_key k_t = Some k) then Some t else None
+  | _ => None
+  end.
+
+Variant open_spec k t : option term → Type :=
+| OpenSome k_t t'
+  of open_key k_t = Some k & t = TSeal k_t t'
+  : open_spec k t (Some t')
+| OpenNone : open_spec k t None.
+
+Lemma openP k t : open_spec k t (open k t).
+Proof.
+case: t; eauto using open_spec => k_t t /=.
+by case: decide => [e|_]; eauto using open_spec.
+Qed.
+
+Definition is_key t :=
+  match t with
+  | TKey kt _ => Some kt
+  | _ => None
+  end.
+
+Variant is_key_spec t : option key_type → Type :=
+| IsKeySome kt k of t = TKey kt k : is_key_spec t (Some kt)
+| IsKeyNone of (∀ kt k, t ≠ TKey kt k) : is_key_spec t None.
+
+Lemma is_keyP t : is_key_spec t (is_key t).
+Proof.
+case: t; try by right.
+by move=> kt t; eleft.
+Qed.
+
+Definition has_key_type kt t :=
+  match is_key t with
+  | Some kt' => bool_decide (kt = kt')
+  | None => false
+  end.
+
+Definition of_list_aux : seal (foldr TPair (TInt 0)). by eexists. Qed.
+Definition of_list := unseal of_list_aux.
+Lemma of_list_unseal : of_list = foldr TPair (TInt 0).
+Proof. exact: seal_eq. Qed.
+
+Lemma of_list_tsize t ts : t ∈ ts → tsize t < tsize (of_list ts).
+Proof.
+rewrite of_list_unseal; elim: ts => [/elem_of_nil |t' ts IH /elem_of_cons] //=.
+rewrite [tsize (TPair _ _)]tsizeE; case=> [<-|/IH t_ts]; lia.
+Qed.
+
+Lemma is_nonce_of_list ts : is_nonce (of_list ts) = false.
+Proof. by rewrite of_list_unseal; case: ts. Qed.
+
+Lemma is_exp_of_list ts : is_exp (of_list ts) = false.
+Proof. by rewrite of_list_unseal; case: ts. Qed.
+
+Fixpoint to_list t : option (list term) :=
+  match t with
+  | TInt 0 => Some []
+  | TPair t1 t2 =>
+    match to_list t2 with
+    | Some l => Some (t1 :: l)
+    | None => None
+    end
+  | _ => None
+  end.
+
+Lemma of_listK l : to_list (of_list l) = Some l.
+Proof. rewrite of_list_unseal; by elim: l => //= t l ->. Qed.
+
+Lemma to_listK t ts :
+  to_list t = Some ts →
+  t = of_list ts.
+Proof.
+rewrite of_list_unseal /=; elim/term_ind': t ts => //.
+  by case=> [] // _ [<-].
+move=> t _ ts' IH /= ts.
+case e: to_list => [ts''|] // [<-].
+by rewrite /= (IH _ e).
+Qed.
+
+Inductive to_list_spec : term → option (list term) → Type :=
+| ToListSome ts : to_list_spec (of_list ts) (Some ts)
+| ToListNone t  : to_list_spec t None.
+
+Lemma to_listP t : to_list_spec t (to_list t).
+Proof.
+case e: to_list => [ts|]; last constructor.
+by rewrite (to_listK e); constructor.
+Qed.
+
+Lemma of_list_inj : Inj eq eq of_list.
+Proof.
+move=> ts1 ts2 e; apply: Some_inj.
+by rewrite -of_listK e of_listK.
+Qed.
+
+Definition enc k c t := TSeal k (tag c t).
+
+Definition dec k c t :=
+  match open k t with
+  | Some t => untag c t
+  | None => None
+  end.
+
+Variant dec_spec k c t : option term → Type :=
+| DecSome k_t t'
+  of open_key k_t = Some k
+  &  t = TSeal k_t (tag c t')
+  : dec_spec k c t (Some t')
+| DecNone : dec_spec k c t None.
+
+Lemma decP k c t : dec_spec k c t (dec k c t).
+Proof.
+rewrite /dec.
+case: openP; eauto using dec_spec.
+move=> {}k_t {}t e ->.
+case: untagP; eauto using dec_spec.
+move=> {}t ->; eauto using dec_spec.
+Qed.
+
+Lemma decK k1 k2 c t t' :
+  open_key k1 = Some k2 →
+  dec k2 c t = Some t' →
+  t = TSeal k1 (tag c t').
+Proof.
+rewrite /Spec.dec /=.
+case: t => [] //= k_t t.
+case: decide => // k_t_k2 k1_k2 /untagK <-.
+rewrite /open_key in k_t_k2 k1_k2.
+case: k_t k1 => [] // kt1 ? [] //= kt2 ? in k_t_k2 k1_k2 *.
+case: kt1 kt2 => [] //= [] //= in k_t_k2 k1_k2 *; congruence.
+Qed.
+
+Definition zero : term := TInt 0.
+
+End Spec.
+
+Arguments repr_term /.
+Arguments Spec.tag_def /.
+Arguments Spec.untag_def /.
+
+#[global]
+Existing Instance Spec.of_list_inj.
+
+Lemma subterm_tag c t1 t2 : subterm t1 t2 → subterm t1 (Spec.tag c t2).
+Proof. by rewrite Spec.tag_unseal; eauto using subterm. Qed.
+
+#[global]
+Hint Resolve STRefl : core.
+
+Global Instance invs_canceled_proper : Proper ((≡ₚ) ==> iff) invs_canceled.
+Proof. move => ts1 ts2 e; exact: perm_invs_canceled. Qed.
+
+Lemma invs_canceled1 t : negb (is_mul t) -> invs_canceled [t].
+Proof. exact: invs_canceled_Nmul1. Qed.
+
+Lemma invs_canceled2 t1 t2 :
+  negb (is_mul t1) -> negb (is_mul t2) ->
+  invs_canceled [t1 ; t2] ↔ (t1 ≠ TInv t2).
+Proof. exact: invs_canceled2_Nmul. Qed.
+
+Lemma exps_TExpN t ts :
+  atomic ts -> exps (TExpN t ts) ≡ₚ cancel_invs (exps t ++ ts).
+Proof.
+move => atom.
+rewrite (exps_TExpN_sort t ts atom).
+exact: (merge_sort_Permutation term_order (cancel_invs (exps t ++ ts))).
+Qed.
+
+(*
+Lemma is_exp_TExpN t ts :
+  is_exp (TExpN t ts) = implb (bool_decide (ts = [])) (is_exp t).
+Proof.
+rewrite is_exp_TExpN -eq_op_bool_decide implb_orb.
+by case: ts.
+Qed.
+*)
+
+Lemma TExp_TExpN t1 ts1 t2 : TExp (TExpN t1 ts1) t2 = TExpN t1 (t2 :: ts1).
+Proof.
+have -> : TExp (TExpN t1 ts1) t2 = TExpN (TExpN t1 ts1) [t2].
+  by rewrite /TExpN TMulN1.
+rewrite TExpNA; apply: TExpN_perm.
+by rewrite -Permutation_cons_append.
+Qed.
+
+Lemma count_exp_TExpNW t1 t2 ts :
+  atomic ts ->
+  (∀ t, t ∈ ts → t1 ≠ TInv t) →
+  (count_exp t1 t2 ≤ count_exp t1 (TExpN t2 ts))%Z.
+Proof.
+elim: ts => [|t ts IH]; first by move => _ _; rewrite TExpN0; lia.
+move => atom t1_ts.
+move: atom => /Forall_cons [Nmt atom'].
+rewrite -TExp_TExpN; set t2' := TExpN t2 ts.
+have ?: (count_exp t1 t2' ≤ count_exp t1 (TExp t2' t))%Z.
+  apply: (count_exp_TExpW Nmt); move/(_ t): t1_ts; apply.
+  rewrite elem_of_cons; by eauto.
+suff: (count_exp t1 t2 ≤ count_exp t1 t2')%Z by lia.
+apply: (IH atom') => t' t'_ts; apply: t1_ts; rewrite elem_of_cons; eauto.
+Qed.
+
+Lemma elem_of_TExpN2l g t1 t2 :
+  negb (is_mul t1) -> negb (is_mul t2) ->
+  t1 ≠ TInv t2 →
+  TInv t1 ∉ exps g →
+  t1 ∈ exps (TExpN g [t1; t2]).
+Proof.
+move=> Nm1 Nm2 t1_t2 t1_g.
+rewrite (not_elem_of_TInv_exps _ Nm1) -count_exp_gt0 in t1_g.
+have e : TExpN g [t1; t2] = TExp (TExp g t1) t2.
+  rewrite (_ : TExp g t1 = TExpN g [t1]); last by rewrite /TExpN TMulN1.
+  rewrite TExp_TExpN; exact: TExpC2.
+rewrite e -count_exp_gt0 (count_exp_TExp t1 (TExp g t1) Nm2).
+rewrite (@decide_False _ (t1 = TInv t2)); last exact: t1_t2.
+by case: decide; lia.
+Qed.
+
+Lemma elem_of_TExpN2r g t1 t2 :
+  negb (is_mul t1) -> negb (is_mul t2) ->
+  t1 ≠ TInv t2 →
+  TInv t2 ∉ exps g →
+  t2 ∈ exps (TExpN g [t1; t2]).
+Proof.
+move=> Nm1 Nm2 t1_t2 t2_g.
+rewrite TExpC2.
+apply: (elem_of_TExpN2l Nm2 Nm1); last exact: t2_g.
+by move=> contra; apply: t1_t2; rewrite contra TInvK.
+Qed.
+
+Lemma base_expN t : ¬ is_exp t → base t = t.
+Proof. move=> tNX; apply: base_expN_bool; apply/negb_True; exact: tNX. Qed.
+
+Lemma exps_expN t : ¬ is_exp t → exps t = [].
+Proof. move=> tNX; apply: exps_expN_bool; apply/negb_True; exact: tNX. Qed.
+
+Lemma exps_TExpN' t ts :
+  ¬ is_exp t -> atomic ts ->
+  invs_canceled ts ->
+  exps (TExpN t ts) ≡ₚ ts.
+Proof.
+move => tNexp atom canc.
+by rewrite (@exps_TExpN t ts atom) (exps_expN tNexp) app_nil_l
+   (cancel_invs_canceled ts atom canc).
+Qed.
+
+Lemma is_exp_base t : ¬ is_exp (base t).
+Proof. apply/negb_True; exact: is_exp_base_bool. Qed.
+Hint Resolve is_exp_base : core.
+
+(* Re-export the [Set Implicit Arguments] argument structure that the old
+   with_stdpp.v restatements provided for these lemmas, so downstream callers
+   that pass only the hypotheses keep working. *)
+Arguments cancel_invs_canceled {ts} _ _.
+Arguments tsize_lt_TExp {t1 t2} _ _.
+Arguments tsize_TExp_TInv {t1 t2} _ _.
